finish proof of body that prints 0 1

iodiv/IIOSigSpec.fst
@@ -15,27 +15,29 @@ open DivFree
 open DivFreeTauSpec
 open DivFreeTauDM
 
-unfold
-let i_open (s : string) : iwp file_descr =
+
+[@@ (postprocess_with (pp_unfold [ `%iprepost ]))]
+unfold let i_open (s : string) : iwp file_descr =
   iprepost (fun _ -> True) (fun hist r -> terminates r /\ ret_trace r == [ EOpenfile s (result r) ])
 
-unfold
-let i_read (fd : file_descr) : iwp string =
+[@@ (postprocess_with (pp_unfold [ `%iprepost ]))]
+unfold let i_read (fd : file_descr) : iwp string =
   iprepost (fun hist -> is_open fd hist) (fun hist r -> terminates r /\ ret_trace r == [ ERead fd (result r) ])
 
-unfold
-let i_print (s : string) : iwp unit =
+[@@ (postprocess_with (pp_unfold [ `%iprepost ]))]
+unfold let i_print (s : string) : iwp unit =
   iprepost (fun hist -> True) (fun hist r -> terminates r /\ ret_trace r == [ EPrint s ])
 
-unfold
-let i_close (fd : file_descr) : iwp unit =
+[@@ (postprocess_with (pp_unfold [ `%iprepost ]))]
+unfold let i_close (fd : file_descr) : iwp unit =
   iprepost (fun hist -> is_open fd hist) (fun hist r -> terminates r /\ ret_trace r == [ EClose fd ])
 
 unfold
 let i_get_trace : iwp history =
   as_iwp (fun post hist -> post (Cv [] hist))
 
-let iodiv_act : action_iwp io_sig =
+unfold
+let i_act : action_iwp io_sig =
   fun ac arg ->
     match ac with
     | Openfile -> i_open arg
@@ -43,8 +45,8 @@ let iodiv_act : action_iwp io_sig =
     | Print -> i_print arg
     | Close -> i_close arg
 
-let iiodiv_act : action_iwp iio_sig =
+let i_iio_call : action_iwp iio_sig =
   fun ac arg ->
     match ac with
     | GetTrace -> i_get_trace
-    | _ -> iodiv_act ac arg
+    | _ -> i_act ac arg
